theories/Examples/Paxos/Consensus.v
@@ -1,5 +1,5 @@
 From VLSM.Lib Require Import Itauto.
-From stdpp Require Import prelude finite base.
+From stdpp Require Import prelude finite.
 From Coq Require Import Streams FunctionalExtensionality Eqdep_dec.
 From VLSM.Lib Require Import Preamble ListExtras.
 From VLSM.Core Require Import VLSM Plans VLSMProjections.
